fomega/Properties.v
@@ -5,11 +5,11 @@ Ltac dauto := try (intros _x; destruct _x; auto).
 
 (* Properties *)
 Lemma renTm_typing : forall Delta Gamma t T,
-  <{ Delta | Gamma |-- t \in T }> ->
+  <[ Delta | Gamma |-- t \in T ]> ->
   forall Gamma' xi,
   (forall x S, nth_error Gamma x = Some S -> 
               nth_error Gamma' (xi x) = Some S) ->
-  <{ Delta | Gamma' |-- {ren_Tm id xi t} \in T }>.
+  <[ Delta | Gamma' |-- {ren_Tm id xi t} \in T ]> .
 Proof.
   intros Delta Gamma t T H.
   induction H; intros; asolve.
@@ -33,11 +33,11 @@ Proof.
 Qed.
 
 Lemma renTy_kinding : forall Delta T K,
-  <{{ Delta |-- T \in K }}> ->
+  <[[ Delta |-- T \in K ]]> ->
   forall Delta' xi,
   (forall X J, nth_error Delta X = Some J -> 
               nth_error Delta' (xi X) = Some J) ->
-  <{{ Delta' |-- {ren_Ty xi T} \in K }}>.
+  <[[ Delta' |-- {ren_Ty xi T} \in K ]]>. 
 Proof.
   intros Delta T K H.
   induction H; intros; asolve;
@@ -48,30 +48,37 @@ Proof.
     intros. destruct X; simpl; auto.
 Qed.
 
-Lemma renTy_tyequiv : forall T1 T2,
-  <{{= T1 = T2 =}}> -> 
+Lemma renTy_tyeval : forall T1 T2, 
+  T1 ==> T2 -> 
   forall xi,
-  <{{= {ren_Ty xi T1} = {ren_Ty xi T2} =}}>.
+  (ren_Ty xi T1) ==> (ren_Ty xi T2).
+Proof.
+  intros T1 T2 H. induction H; intros; asolve;
+  try (constructor; apply IHtype_eval_step).
+  - subst S. asolve. apply TST_Red. asolve.
+    apply ext_Ty. intros. unfold sigma_ty_one. destruct x; asolve.  
+Qed.
+
+Lemma renTy_tyeq : forall T1 T2,
+  T1 === T2 -> 
+  forall xi,
+  (ren_Ty xi T1) === (ren_Ty xi T2).
 Proof.
   intros T1 T2 H. induction H; intros; asolve.
-  - apply TQ_Refl.
-  - apply TQ_Sym. auto.
-  - eapply TQ_Trans; auto.
-  - eapply TQ_Abs. auto.
-  - apply TQ_App; auto.
-  - apply TQ_Arr; auto.
-  - apply TQ_All; auto.
-  - apply TQ_Unit.
-Qed. 
-
+  - apply multi_refl.
+  - apply multi_step with (T2:=ren_Ty xi T2).
+    + destruct H; [left | right]; apply renTy_tyeval; assumption.
+    + apply IHmulti.
+Qed.
+  
 Lemma renTy_typing : forall Delta Gamma t T,
-  <{ Delta | Gamma |-- t \in T }> ->
+  <[ Delta | Gamma |-- t \in T ]> ->
   forall Gamma' Delta' xi,
   (forall x S, nth_error Gamma x = Some S -> 
               nth_error Gamma' x = Some (ren_Ty xi S)) ->
   (forall X K, nth_error Delta X = Some K -> 
               nth_error Delta' (xi X) = Some K) ->
-  <{ Delta' | Gamma' |-- {ren_Tm xi id t} \in {ren_Ty xi T} }>.
+  <[ Delta' | Gamma' |-- {ren_Tm xi id t} \in {ren_Ty xi T} ]>.
 Proof.
   intros Delta Gamma t T H.
   induction H; intros Gamma' Delta' xi HG HD; asolve.
@@ -106,16 +113,16 @@ Proof.
     + eapply renTy_kinding; eassumption.
   - eapply T_Conv.
     + apply IHhas_type; assumption.
-    + apply renTy_tyequiv. assumption.
+    + apply renTy_tyeq. assumption.
   - apply T_Unit.
 Qed.
 
 Lemma tmsubst_preserves_typing :
   forall Delta Gamma t T,
-  <{ Delta | Gamma |-- t \in T }> ->
+  <[ Delta | Gamma |-- t \in T ]> ->
   forall Gamma' sigma,
-  (forall x S, nth_error Gamma x = Some S -> <{ Delta | Gamma' |-- {sigma x} \in S }>) ->
-  <{ Delta | Gamma' |-- {subst_Tm id sigma t} \in T }>.
+  (forall x S, nth_error Gamma x = Some S -> <[ Delta | Gamma' |-- {sigma x} \in S ]>) ->
+  <[ Delta | Gamma' |-- {subst_Tm id sigma t} \in T ]>.
 Proof.
   intros Delta Gamma t T.
   intro H. induction H; intros; asolve.
@@ -143,3 +150,324 @@ Proof.
     apply IHhas_type. assumption.
   - constructor.
 Qed.
+
+Lemma tysubst_preserves_kinding : 
+  forall Delta T K,
+  <[[ Delta |-- T \in K ]]> ->
+  forall sigma Delta',
+  ( forall X J, nth_error Delta X = Some J ->
+    <[[ Delta' |-- {sigma X} \in J ]]> ) ->
+  <[[ Delta' |-- {subst_Ty sigma T} \in K ]]>. 
+Proof.
+  intros Delta T K H.
+  induction H; intros; asolve.
+  - apply K_Abs. apply IHhas_kind. intros.
+    destruct X.
+    + apply K_TVar. assumption.
+    + apply renTy_kinding with Delta'.
+      * apply H0. assumption.
+      * intros. assumption.
+  - apply K_App with K2.
+    + apply IHhas_kind1. assumption.
+    + apply IHhas_kind2. assumption.
+  - apply K_Arr.
+    + apply IHhas_kind1. assumption.
+    + apply IHhas_kind2. assumption.
+  - apply K_All. apply IHhas_kind.
+    intros. destruct X.
+    + apply K_TVar. assumption.
+    + apply renTy_kinding with Delta'.
+      * apply H0. assumption.
+      * intros. assumption.
+  - apply K_Unit.
+Qed.
+
+Lemma tysubst_preserves_tyeval : 
+  forall T1 T2,
+  T1 ==> T2 ->
+  forall sigma,
+  (subst_Ty sigma T1) ==> (subst_Ty sigma T2).
+Proof.
+  intros T1 T2 H. induction H; intros; asolve;
+  try (constructor; apply IHtype_eval_step).
+  - subst S. apply TST_Red. asolve. unfold sigma_ty_one.
+    apply ext_Ty. intros. asolve. destruct x; asolve.
+    + apply ext_Ty. intros x. rewrite renRen_Ty. asolve.
+    + rewrite idSubst_Ty; auto.
+Qed.
+
+Lemma tysubst_preserves_tyeq : 
+  forall T1 T2,
+  T1 === T2 ->
+  forall sigma,
+  (subst_Ty sigma T1) === (subst_Ty sigma T2).
+Proof.
+  intros T1 T2 H. induction H; intros.
+  - apply multi_refl.
+  - apply multi_step with (T2:=subst_Ty sigma T2).
+    + destruct H; [left|right]; apply tysubst_preserves_tyeval;
+      assumption.
+    + apply IHmulti.
+Qed.
+
+Lemma tysubst_preserves_typing :
+  forall Delta Gamma t T, 
+  <[ Delta | Gamma |-- t \in T ]> ->
+  forall sigma Gamma',
+  ( forall x U, nth_error Gamma x = Some U ->
+    nth_error Gamma' x = Some (subst_Ty sigma U) ) ->
+  forall Delta',
+  ( forall X K, nth_error Delta X = Some K ->
+    <[[ Delta' |-- {sigma X} \in K ]]> ) ->
+  <[ Delta' | Gamma' |-- {subst_Tm sigma id t} \in {subst_Ty sigma T} ]>.
+Proof.
+  intros Delta Gamma t T H.
+  induction H; intros sigma Gamma' HG Delta' HD; asolve.
+  - apply T_Var. apply HG. apply H.
+  - apply T_Abs.
+    + apply tysubst_preserves_kinding with Delta; assumption.
+    + asimpl. rewrite ext_Tm with (tau_Ty:=sigma) (tau_Tm:=id).
+      * apply IHhas_type.
+        { intros. destruct x.
+          - simpl. inversion H1. reflexivity.
+          - simpl. simpl in H1. apply HG. assumption. }
+        { assumption. }
+      * reflexivity.
+      * intro x. destruct x; auto.
+  - apply T_App with (subst_Ty sigma T1).
+    + apply IHhas_type1; assumption.
+    + apply IHhas_type2; assumption.
+  - apply T_TAbs with (map (ren_Ty S) Gamma'); try reflexivity.
+    subst GammaS. apply IHhas_type.
+    + intros. rewrite nth_error_map in *.
+      destruct (nth_error Gamma x) as [U'|] eqn: EqGx; try discriminate.
+      simpl in H0. rewrite (HG x U' EqGx). simpl. f_equal.
+      inversion H0. asolve.
+    + intros. destruct X.
+      * apply K_TVar. assumption.
+      * apply renTy_kinding with Delta'.
+        { apply HD. assumption. }
+        { intros. assumption. }
+  - apply T_TApp with (K:=K) (T1:=(subst_Ty (up_Ty_Ty sigma) T1)).
+    + apply IHhas_type.
+      * intros. apply HG. assumption.
+      * assumption.
+    + subst T1'. asolve. apply ext_Ty. intros.
+      destruct x; asolve.
+      symmetry. apply idSubst_Ty. reflexivity.
+    + apply tysubst_preserves_kinding with Delta; assumption.
+  - eapply T_Conv.
+    + apply IHhas_type; assumption.
+    + apply tysubst_preserves_tyeq. assumption. 
+  - apply T_Unit.
+Qed.
+
+Lemma multi_append : 
+  forall X R (S T U: X), (multi R S T) /\ (R T U) -> (multi R S U).
+Proof.
+  intros. destruct H. generalize dependent U.
+  induction H; intros.
+  - apply multi_step with U.
+    + assumption.
+    + apply multi_refl.
+  - apply multi_step with T2.
+    + assumption.
+    + apply IHmulti. assumption.
+Qed.
+
+Definition tyeval_append := multi_append Ty type_eval_step.
+Definition tyeq_append := multi_append Ty type_eval_step_lr.
+
+Lemma tyeq_sym :
+  forall S T, S === T -> T === S.
+Proof.
+  intros. induction H.
+  - apply multi_refl.
+  - apply tyeq_append with T2. split.
+    + assumption.
+    + destruct H; [right | left]; assumption.
+Qed.
+
+Lemma tyeq_trans :
+  forall S T U, (S === U) /\ (U === T) -> S === T.
+Proof.
+  intros. destruct H as [HS HT].
+  generalize dependent T. induction HS; intros U H1.
+  - assumption.
+  - apply multi_step with T2.
+    + assumption.
+    + apply IHHS. assumption.
+Qed.
+
+Lemma multi_step_implies_tyeq : 
+  forall S T, multi type_eval_step S T -> S === T.
+Proof.
+  intros. induction H.
+  - apply multi_refl.
+  - apply multi_step with T2.
+    + left. assumption.
+    + apply IHmulti.
+Qed.
+
+Lemma equivalent_types_have_same_contractum: 
+  forall S T,
+  S === T ->
+  exists U, ((multi type_eval_step S U) /\ (multi type_eval_step T U)).
+Proof.
+  intros. induction H.
+  - exists T. split; apply multi_refl.
+  - destruct IHmulti as [U' [IHT2 IHT3] ]. destruct H.
+    + exists U'. split.
+      * apply multi_step with T2; assumption.
+      * assumption.
+    + inversion IHT2.
+      * subst U'. exists T1. split.
+        { apply multi_refl. }
+        { apply tyeval_append with T2. split; assumption. }
+      * replace T4 with T1 in *.
+        { exists U'. split; assumption. }
+        { admit. }
+Admitted.
+
+Lemma confluence_implies_tyeq : 
+  forall S T U,
+  multi type_eval_step S U /\ multi type_eval_step T U ->
+  S === T.
+Proof.
+  intros. destruct H as [HS HT]. induction HS.
+  - apply tyeq_sym. apply multi_step_implies_tyeq. assumption.
+  - apply multi_step with T2.
+    + left. assumption.
+    + apply IHHS. assumption.
+Qed.
+
+(* TmAbs invesion *)
+Lemma tyeval_preserves_type_form_fun :
+  forall S1 S2 T, 
+  multi type_eval_step <{{S1 -> S2}}> T ->
+  exists T1 T2,
+  T = <{{T1 -> T2}}> /\ (multi type_eval_step S1 T1) /\ (multi type_eval_step S2 T2).
+Proof.
+  intros. remember <{{S1 -> S2}}> as S.
+  generalize dependent HeqS. generalize dependent S2. generalize dependent S1.
+  induction H; intros.
+  - exists S1, S2; repeat split; try assumption; apply multi_refl.
+  - rename T1 into S, T2 into U, T3 into T.
+    subst S. inversion H.
+    + rename S0 into U1. symmetry in H2. subst T1 T2.
+      apply IHmulti in H2 as [T1 [T2 [HT [H1 H2] ] ] ].
+      exists T1, T2. repeat split; try assumption.
+      * apply multi_step with U1; assumption. 
+    + rename S0 into U2. symmetry in H2. subst T1 T2.
+      apply IHmulti in H2 as [T1 [T2 [HT [H1 H2] ] ] ].
+      exists T1, T2. repeat split; try assumption.
+      * apply multi_step with U2; assumption.
+Qed.
+
+Lemma invert_tyeq_fun : 
+  forall S1 S2 T1 T2, 
+  <{{S1 -> S2}}> === <{{T1 -> T2}}> ->
+  (S1 === T1) /\ (S2 === T2).
+Proof.
+  intros. apply equivalent_types_have_same_contractum in H as [U [H1 H2] ]. 
+  apply tyeval_preserves_type_form_fun in H1 as [U1 [U2 [HU [H11 H12] ] ] ].
+  apply tyeval_preserves_type_form_fun in H2 as [V1 [V2 [HV [H21 H22] ] ] ].
+  subst U. inversion HV. subst V1 V2. clear HV. split;
+  eapply confluence_implies_tyeq; split; eassumption.
+Qed.
+
+Lemma invert_typing_abs :
+  forall Delta Gamma S1 t1 T,
+  <[ Delta | Gamma |-- \:S1, t1 \in T ]> ->
+  forall T1 T2,
+  T === <{{ T1 -> T2 }}> ->
+  (S1 === T1) /\ <[ Delta | S1 :: Gamma |-- t1 \in T2 ]>.
+Proof.
+  intros Delta Gamma S1 t1 T H. 
+  remember <{ \:S1, t1 }> as t.
+  generalize dependent Heqt.
+  induction H; try discriminate; intros.
+  - apply invert_tyeq_fun in H1 as [Hl Hr].
+    inversion Heqt. subst. split. 
+    + assumption.
+    + eapply T_Conv; eassumption.
+  - apply IHhas_type.
+    + assumption.
+    + eapply tyeq_trans. split; eassumption.
+Qed.
+
+
+(* TmTAbs inversion *)
+Lemma invert_typing_tyabs :   
+  forall Delta Gamma J t1 T,
+  <[ Delta | Gamma |-- \::J, t1 \in T ]> ->
+  forall K T1,
+  T === <{{ -/::K, T1 }}> ->
+  K = J /\ <[ J :: Delta | map (ren_Ty S) Gamma |-- t1 \in T1 ]>.
+Proof.
+  intros Delta Gamma J t1 T H. 
+  remember <{ \::J, t1 }> as t.
+  generalize dependent Heqt.
+  induction H; try discriminate; intros.
+  - assert ( T1 === T0 ). { admit. }
+    assert (K = K0). { admit. }
+    + inversion Heqt. subst. split. 
+      * reflexivity.
+      * eapply T_Conv; eassumption.
+  - apply IHhas_type.
+    + assumption.
+    + eapply tyeq_trans. split; eassumption.
+Admitted.
+
+
+Theorem preservation :
+  forall Delta Gamma t T,
+  <[ Delta | Gamma |-- t \in T ]> ->
+  forall t',
+  t --> t' ->
+  <[ Delta | Gamma |-- t' \in T ]>.
+Proof.
+  intros Delta Gamma t T H. induction H; intros.
+  - inversion H0.
+  - inversion H1.
+  - inversion H1.
+    + asolve. unfold sigma_tm_one. subst t1.
+      apply invert_typing_abs with (T1:=T1) (T2:=T2) in H as [HT1 Ht].
+      * apply tmsubst_preserves_typing with (Gamma:=(T::Gamma)).
+        { apply Ht. }
+        { intros. destruct x; simpl.
+          - rewrite renRen_Tm. asolve.
+            simpl in H. inversion H. subst S. 
+            eapply T_Conv.
+            + eassumption.
+            + apply tyeq_sym; assumption.
+          - apply T_Var. assumption. }
+      * apply multi_refl. 
+    + apply T_App with T1.
+      * apply IHhas_type1. assumption.
+      * assumption.
+    + apply T_App with T1.
+      * assumption.
+      * apply IHhas_type2. assumption.
+  - inversion H1.
+  - inversion H2.
+    + subst. asolve. unfold sigma_ty_one.
+      apply invert_typing_tyabs with (K:=K) (T1:=T1) in H as [HK Ht].
+      * eapply tysubst_preserves_typing.
+        { apply Ht. }
+        { intros. rewrite nth_error_map in H.
+          destruct (nth_error Gamma x) as [V|]; try discriminate.
+          simpl in H. inversion H.
+          f_equal. asolve. rewrite idSubst_Ty; try reflexivity. }
+        { intros. destruct X; simpl. 
+          - rewrite renRen_Ty. asolve. simpl in H. inversion H. subst.
+            assumption. 
+          - apply K_TVar. assumption. }
+      * apply multi_refl.
+    + eapply T_TApp; try eassumption.
+      * apply IHhas_type. assumption.
+  - eapply T_Conv.
+    + apply IHhas_type. assumption.
+    + assumption.
+  - inversion H.
+Qed. 
